progress

src/Utilities/FisherYates/Implementation.dfy
@@ -10,26 +10,31 @@ module FisherYates.Implementation {
   import Permutations
   import Helper
   import Monad
+  import Equivalence
 
   trait {:termination false} Trait extends Interface.Trait {
 
-    method Shuffle<T>(a: array<T>)
+    method Shuffle<T(!new)>(a: array<T>)
       modifies this, a
       decreases *
-      ensures Model.Shuffle(Helper.ArrayToSeq(old(a)))(old(s)) == Monad.Result(Helper.ArrayToSeq(a), s)
+      ensures Model.Shuffle(old(Helper.ArrayToSeq(a)))(old(s)) == Monad.Result(Helper.ArrayToSeq(a), s)
     {
-      var i := 0;
-      while i < a.Length 
-        invariant 0 <= i <= a.Length
-        invariant Model.Shuffle(old(Helper.ArrayToSeq(a)))(old(s)) == Model.Shuffle(Helper.ArrayToSeq(a), i)(s)
-      {
+      var i := 0; 
+
+      while i < a.Length
+        decreases a.Length - i
+        invariant i <= a.Length
+        invariant Model.ShuffleLoop(old(Helper.ArrayToSeq(a)))(old(s)) == Model.ShuffleLoop(Helper.ArrayToSeq(a), i)(s)
+      {        
         assume {:axiom} false;
-        assert 0 <= i < a.Length;
+        Equivalence.ShuffleLoopTailRecursiveEquivalence(Helper.ArrayToSeq(a), s, i);
+
         var j := UniformIntervalSample(i, a.Length);
-        assert i <= j < a.Length;
         Swap(a, i, j);
         i := i + 1;
       }
+
+      Equivalence.ShuffleLiftToEnsures(old(s), s, old(Helper.ArrayToSeq(a)), Helper.ArrayToSeq(a), i);
     }
 
     method Swap<T>(a: array<T>, i: nat, j: nat)
