src/Utilities/FisherYates/Equivalence.dfy
@@ -4,5 +4,114 @@
  *******************************************************************************/
 
 module FisherYates.Equivalence {
+  import Model 
+  import Rand
+  import Monad
+  import Uniform
+  import Permutations
+  import Loops
 
+  lemma ShuffleLoopTailRecursiveEquivalence<T(!new)>(xs: seq<T>, s: Rand.Bitstream, i: nat := 0)
+    requires 0 <= i <= |xs|
+    ensures 
+      Model.ShuffleLoop(xs)(s) ==
+        if i < |xs| then
+          Monad.Bind(
+            Uniform.Model.IntervalSample(i, |xs|),
+            (j: int) requires i <= j < |xs| => 
+              var xs := Permutations.Swap(xs, 0, j);
+              Model.ShuffleLoop(xs, i + 1)
+          )(s)
+        else 
+          Monad.Return((xs, i))(s)
+  {
+    calc {
+      Model.ShuffleLoop(xs, i)(s);
+    == { reveal Model.ShuffleLoop(); 
+         reveal Model.ShuffleWhileLoopCondition();
+         reveal Model.ShuffleWhileLoopBody();
+         reveal Loops.While(); }
+      Loops.While(Model.ShuffleWhileLoopCondition, Model.ShuffleWhileLoopBody)((xs, i))(s);
+    == { Model.ShuffleTerminatesAlmostSurely<T>();
+         Loops.WhileUnroll(Model.ShuffleWhileLoopCondition, Model.ShuffleWhileLoopBody, (xs, i), s); 
+         reveal Model.ShuffleWhileLoopCondition();
+         reveal Model.ShuffleWhileLoopBody(); 
+         reveal Model.ShuffleLoop(); }
+      if Model.ShuffleWhileLoopCondition((xs, i)) then 
+        Monad.Bind(
+          Model.ShuffleWhileLoopBody((xs, i)),
+          (xsI: (seq<T>, nat)) => Model.ShuffleLoop(xsI.0, xsI.1)
+        )(s)
+      else 
+        Monad.Return((xs, i))(s);
+    == { reveal Model.ShuffleWhileLoopBody(); 
+         reveal Model.ShuffleWhileLoopCondition(); 
+         reveal Model.ShuffleLoop(); }
+      if i < |xs| then 
+        Monad.Bind<(seq<T>, nat), (seq<T>, nat)>(
+          Monad.Bind<int, (seq<T>, nat)>(
+            Uniform.Model.IntervalSample(i as int, |xs| as int),
+            (j: int) requires i as int <= j < |xs| as int => 
+              var xs := Permutations.Swap(xs, i, j as nat); 
+              Monad.Return((xs, i + 1 as nat))
+          ),
+          (xsI: (seq<T>, nat)) => Model.ShuffleLoop(xsI.0, xsI.1)
+        )(s)
+      else 
+        Monad.Return((xs, i))(s);  
+    ==
+      if i < |xs| then 
+        Monad.Bind<int, (seq<T>, nat)>(
+          Uniform.Model.IntervalSample(i as int, |xs| as int),
+          (j: int) requires i as int <= j < |xs| as int => 
+            var xs := Permutations.Swap(xs, i, j as nat); 
+            Monad.Bind<(seq<T>, nat), (seq<T>, nat)>(
+              Monad.Return((xs, i + 1 as nat)),
+              (xsI: (seq<T>, nat)) => Model.ShuffleLoop(xsI.0, xsI.1)
+            )
+        )(s)
+      else 
+        Monad.Return((xs, i))(s);  
+  == { forall xsI: (seq<T>, nat), s: Rand.Bitstream { Monad.UnitalityBindReturn(xsI, (xsI: (seq<T>, nat)) => Model.ShuffleLoop(xsI.0, xsI.1), s); } }
+      if i < |xs| then
+        Monad.Bind<int, (seq<T>, nat)>(
+          Uniform.Model.IntervalSample(i as int, |xs| as int),
+          (j: int) requires i as int <= j < |xs| as int => 
+            var xs := Permutations.Swap(xs, i, j as nat);
+            Model.ShuffleLoop(xs, i + 1 as nat)
+        )(s)
+      else 
+        Monad.Return((xs, i))(s);
+    }
+  }
+
+
+  lemma ShuffleLiftToEnsures<T(!new)>(s: Rand.Bitstream, t: Rand.Bitstream, xs: seq<T>, ys: seq<T>, i: nat)
+    requires R1: Model.ShuffleLoop(xs)(s) == Model.ShuffleLoop(ys, i)(t)
+    requires R2: i == |ys|
+    ensures Model.Shuffle(xs)(s) == Monad.Result(ys, t)
+  {
+    var f := (xsI: (seq<T>, nat)) => xsI.0;
+
+    calc {
+      Model.Shuffle(xs)(s);
+      { reveal Model.Shuffle(); }
+      Monad.Map(Model.ShuffleLoop(xs), f)(s);
+      Model.ShuffleLoop(xs)(s).Map(f);
+      { reveal R1; }
+      Model.ShuffleLoop(ys, i)(t).Map(f);
+      { reveal Model.ShuffleLoop(); 
+        reveal Model.ShuffleWhileLoopCondition(); 
+        reveal Model.ShuffleWhileLoopBody(); }
+      Loops.While(Model.ShuffleWhileLoopCondition, Model.ShuffleWhileLoopBody)((ys, i))(t).Map(f);
+      { reveal Model.ShuffleWhileLoopCondition(); }
+      Loops.While((xsI: (seq<T>, nat)) => xsI.1 < |xsI.0|, Model.ShuffleWhileLoopBody)((ys, i))(t).Map(f);
+      { reveal Loops.While(); 
+        reveal R2; }
+      Monad.Return((ys, i))(t).Map(f);
+      Monad.Result((ys, i), t).Map(f);
+      Monad.Result(f((ys, i)), t);
+      Monad.Result(ys, t);
+    }
+  }
 }
